Add support for more assembly
I want to be able to handle the output of gcc/clang on our C code.

Right now, I have added support for parsing the assembly output.
Equivalence checking is still to come.

src/Assembly/Parse/Examples/fiat_25519_all_clang_19_1_0_O1.s
@@ -1,0 +1,905 @@
+_Z24fiat_25519_addcarryx_u51PmPhhmm:
+        mov     eax, edx
+        add     rcx, r8
+        add     rcx, rax
+        movabs  rax, 2251799813685247
+        and     rax, rcx
+        shr     rcx, 51
+        mov     qword ptr [rdi], rax
+        mov     byte ptr [rsi], cl
+        ret
+
+_Z25fiat_25519_subborrowx_u51PmPhhmm:
+        mov     eax, edx
+        add     rax, r8
+        sub     rcx, rax
+        movabs  rax, 2251799813685247
+        and     rax, rcx
+        mov     qword ptr [rdi], rax
+        shr     rcx, 51
+        neg     cl
+        mov     byte ptr [rsi], cl
+        ret
+
+_Z22fiat_25519_cmovznz_u64Pmhmm:
+        test    esi, esi
+        cmovne  rdx, rcx
+        mov     qword ptr [rdi], rdx
+        ret
+
+_Z20fiat_25519_carry_mulPmPKmS1_:
+        push    rbp
+        push    r15
+        push    r14
+        push    r13
+        push    r12
+        push    rbx
+        sub     rsp, 192
+        mov     r8, rdx
+        mov     r15, qword ptr [rsi + 32]
+        mov     r13, rsi
+        mov     qword ptr [rsp - 104], rsi
+        mov     rcx, qword ptr [rdx + 32]
+        mov     qword ptr [rsp - 96], rcx
+        lea     rax, [rcx + 8*rcx]
+        lea     rbx, [rcx + 2*rax]
+        mov     rax, rbx
+        mul     r15
+        mov     qword ptr [rsp + 176], rax
+        mov     qword ptr [rsp + 184], rdx
+        mov     rcx, qword ptr [r8 + 24]
+        mov     qword ptr [rsp - 120], rcx
+        lea     rax, [rcx + 8*rcx]
+        lea     r9, [rcx + 2*rax]
+        mov     rax, r9
+        mul     r15
+        mov     qword ptr [rsp + 144], rax
+        mov     qword ptr [rsp + 152], rdx
+        mov     rcx, qword ptr [r8 + 16]
+        mov     qword ptr [rsp - 128], rcx
+        lea     rax, [rcx + 8*rcx]
+        lea     r10, [rcx + 2*rax]
+        mov     rax, r10
+        mul     r15
+        mov     qword ptr [rsp + 128], rax
+        mov     qword ptr [rsp + 136], rdx
+        mov     rcx, qword ptr [r8 + 8]
+        lea     rax, [rcx + 8*rcx]
+        lea     rax, [rcx + 2*rax]
+        mul     r15
+        mov     qword ptr [rsp + 56], rax
+        mov     qword ptr [rsp + 64], rdx
+        mov     r14, qword ptr [rsi + 24]
+        mov     rax, r14
+        mul     rbx
+        mov     r11, rdx
+        mov     qword ptr [rsp + 40], rax
+        mov     rax, r14
+        mul     r9
+        mov     rbp, rdx
+        mov     rsi, rax
+        mov     rax, r14
+        mul     r10
+        mov     qword ptr [rsp + 16], rax
+        mov     r12, rdx
+        mov     r10, qword ptr [r13 + 16]
+        mov     rax, r10
+        mul     rbx
+        mov     qword ptr [rsp + 72], rdx
+        mov     qword ptr [rsp + 48], rax
+        mov     rax, r10
+        mul     r9
+        mov     qword ptr [rsp - 16], rax
+        mov     qword ptr [rsp - 8], rdx
+        mov     r9, qword ptr [r13 + 8]
+        mov     rax, r9
+        mul     rbx
+        mov     qword ptr [rsp - 32], rax
+        mov     qword ptr [rsp - 24], rdx
+        mov     r8, qword ptr [r8]
+        mov     rax, r8
+        mul     r15
+        mov     qword ptr [rsp + 168], rdx
+        mov     qword ptr [rsp + 160], rax
+        mov     rax, r14
+        mov     r15, rcx
+        mov     qword ptr [rsp - 112], rcx
+        mul     rcx
+        mov     qword ptr [rsp + 120], rdx
+        mov     qword ptr [rsp + 112], rax
+        mov     rax, r8
+        mov     qword ptr [rsp - 88], r8
+        mul     r14
+        mov     qword ptr [rsp + 104], rdx
+        mov     qword ptr [rsp + 96], rax
+        mov     rax, r10
+        mov     rcx, qword ptr [rsp - 128]
+        mul     rcx
+        mov     r13, rdx
+        mov     rbx, rax
+        mov     rax, r10
+        mul     r15
+        mov     r15, rdx
+        mov     r14, rax
+        mov     rax, r8
+        mul     r10
+        mov     qword ptr [rsp + 8], rdx
+        mov     qword ptr [rsp], rax
+        mov     rax, r9
+        mul     qword ptr [rsp - 120]
+        mov     qword ptr [rsp + 88], rdx
+        mov     qword ptr [rsp + 80], rax
+        mov     rax, r9
+        mul     rcx
+        mov     qword ptr [rsp + 32], rdx
+        mov     qword ptr [rsp + 24], rax
+        mov     rax, r9
+        mov     r8, qword ptr [rsp - 112]
+        mul     r8
+        mov     qword ptr [rsp - 56], rax
+        mov     qword ptr [rsp - 48], rdx
+        mov     rax, qword ptr [rsp - 104]
+        mov     r10, qword ptr [rax]
+        mov     rcx, qword ptr [rsp - 88]
+        mov     rax, rcx
+        mul     r9
+        mov     qword ptr [rsp - 72], rdx
+        mov     qword ptr [rsp - 80], rax
+        mov     rax, r10
+        mul     qword ptr [rsp - 96]
+        mov     qword ptr [rsp - 96], rdx
+        mov     qword ptr [rsp - 104], rax
+        mov     rax, r10
+        mul     qword ptr [rsp - 120]
+        mov     qword ptr [rsp - 120], rdx
+        mov     qword ptr [rsp - 40], rax
+        mov     rax, r10
+        mul     qword ptr [rsp - 128]
+        mov     qword ptr [rsp - 128], rdx
+        mov     qword ptr [rsp - 64], rax
+        mov     rax, r10
+        mul     r8
+        mov     qword ptr [rsp - 112], rdx
+        mov     r9, rax
+        mov     rax, r10
+        mul     rcx
+        mov     r8, qword ptr [rsp + 16]
+        add     r8, qword ptr [rsp + 56]
+        adc     r12, qword ptr [rsp + 64]
+        add     r8, qword ptr [rsp - 16]
+        adc     r12, qword ptr [rsp - 8]
+        add     r8, qword ptr [rsp - 32]
+        adc     r12, qword ptr [rsp - 24]
+        add     r8, rax
+        adc     r12, rdx
+        shld    r12, r8, 13
+        movabs  rax, 2251799813685247
+        and     r8, rax
+        mov     rcx, qword ptr [rsp + 40]
+        add     rcx, qword ptr [rsp + 144]
+        adc     r11, qword ptr [rsp + 152]
+        add     rsi, qword ptr [rsp + 128]
+        adc     rbp, qword ptr [rsp + 136]
+        add     rsi, qword ptr [rsp + 48]
+        adc     rbp, qword ptr [rsp + 72]
+        add     rsi, qword ptr [rsp - 80]
+        adc     rbp, qword ptr [rsp - 72]
+        add     rsi, r9
+        adc     rbp, qword ptr [rsp - 112]
+        add     rsi, r12
+        adc     rbp, 0
+        shld    rbp, rsi, 13
+        and     rsi, rax
+        add     rcx, qword ptr [rsp - 56]
+        adc     r11, qword ptr [rsp - 48]
+        add     rcx, qword ptr [rsp]
+        adc     r11, qword ptr [rsp + 8]
+        add     rcx, qword ptr [rsp - 64]
+        adc     r11, qword ptr [rsp - 128]
+        add     rcx, rbp
+        adc     r11, 0
+        shld    r11, rcx, 13
+        and     rcx, rax
+        add     r14, qword ptr [rsp + 176]
+        adc     r15, qword ptr [rsp + 184]
+        add     r14, qword ptr [rsp + 24]
+        adc     r15, qword ptr [rsp + 32]
+        add     r14, qword ptr [rsp + 96]
+        adc     r15, qword ptr [rsp + 104]
+        add     r14, qword ptr [rsp - 40]
+        adc     r15, qword ptr [rsp - 120]
+        add     r14, r11
+        adc     r15, 0
+        shld    r15, r14, 13
+        and     r14, rax
+        add     rbx, qword ptr [rsp + 112]
+        adc     r13, qword ptr [rsp + 120]
+        add     rbx, qword ptr [rsp + 80]
+        adc     r13, qword ptr [rsp + 88]
+        add     rbx, qword ptr [rsp + 160]
+        adc     r13, qword ptr [rsp + 168]
+        add     rbx, qword ptr [rsp - 104]
+        adc     r13, qword ptr [rsp - 96]
+        add     rbx, r15
+        adc     r13, 0
+        shld    r13, rbx, 13
+        lea     rdx, [8*r13]
+        add     rdx, r13
+        lea     rdx, [2*rdx]
+        add     rdx, r13
+        add     rdx, r8
+        mov     r8, rdx
+        shr     r8, 51
+        add     r8, rsi
+        mov     rsi, r8
+        shr     rsi, 51
+        add     rsi, rcx
+        and     rbx, rax
+        and     rdx, rax
+        and     r8, rax
+        mov     qword ptr [rdi], rdx
+        mov     qword ptr [rdi + 8], r8
+        mov     qword ptr [rdi + 16], rsi
+        mov     qword ptr [rdi + 24], r14
+        mov     qword ptr [rdi + 32], rbx
+        add     rsp, 192
+        pop     rbx
+        pop     r12
+        pop     r13
+        pop     r14
+        pop     r15
+        pop     rbp
+        ret
+
+_Z23fiat_25519_carry_squarePmPKm:
+        push    rbp
+        push    r15
+        push    r14
+        push    r13
+        push    r12
+        push    rbx
+        push    rax
+        mov     rdx, qword ptr [rsi + 32]
+        lea     rax, [rdx + 8*rdx]
+        lea     rax, [rdx + 2*rax]
+        imul    r10, rdx, 38
+        lea     rcx, [rdx + rdx]
+        mov     qword ptr [rsp - 112], rcx
+        mov     r8, qword ptr [rsi + 24]
+        lea     rcx, [r8 + 8*r8]
+        lea     rcx, [r8 + 2*rcx]
+        imul    r11, r8, 38
+        mul     rdx
+        mov     qword ptr [rsp - 32], rax
+        mov     qword ptr [rsp - 24], rdx
+        mov     r9, qword ptr [rsi + 16]
+        mov     rax, r8
+        mul     r10
+        mov     qword ptr [rsp - 8], rdx
+        mov     qword ptr [rsp - 40], rax
+        mov     rax, rcx
+        mul     r8
+        mov     qword ptr [rsp], rdx
+        mov     qword ptr [rsp - 16], rax
+        mov     rax, r9
+        mul     r10
+        mov     rbx, rax
+        mov     rcx, rdx
+        add     r8, r8
+        mov     qword ptr [rsp - 128], r8
+        mov     rax, r9
+        mul     r11
+        mov     qword ptr [rsp - 72], rax
+        mov     qword ptr [rsp - 64], rdx
+        lea     r14, [r9 + r9]
+        mov     qword ptr [rsp - 120], r14
+        mov     rax, r9
+        mul     r9
+        mov     qword ptr [rsp - 56], rax
+        mov     qword ptr [rsp - 48], rdx
+        mov     rbp, qword ptr [rsi + 8]
+        mov     rax, rbp
+        mul     r10
+        mov     r15, rdx
+        mov     r9, rax
+        mov     rax, rbp
+        mul     r8
+        mov     r11, rdx
+        mov     r13, rax
+        mov     rax, rbp
+        mul     r14
+        mov     r14, rax
+        mov     r8, rdx
+        mov     rsi, qword ptr [rsi]
+        mov     rax, rbp
+        mul     rbp
+        mov     r10, rdx
+        mov     r12, rax
+        mov     rax, rsi
+        mul     qword ptr [rsp - 112]
+        mov     qword ptr [rsp - 80], rdx
+        mov     qword ptr [rsp - 104], rax
+        mov     rax, rsi
+        mul     qword ptr [rsp - 128]
+        mov     qword ptr [rsp - 88], rax
+        mov     qword ptr [rsp - 128], rdx
+        add     rbp, rbp
+        mov     rax, rsi
+        mul     qword ptr [rsp - 120]
+        mov     qword ptr [rsp - 112], rdx
+        mov     qword ptr [rsp - 96], rax
+        mov     rax, rsi
+        mul     rbp
+        mov     rbp, rdx
+        mov     qword ptr [rsp - 120], rax
+        mov     rax, rsi
+        mul     rsi
+        add     r9, qword ptr [rsp - 72]
+        adc     r15, qword ptr [rsp - 64]
+        add     r9, rax
+        adc     r15, rdx
+        shld    r15, r9, 13
+        movabs  rax, 2251799813685247
+        and     r9, rax
+        add     r13, qword ptr [rsp - 56]
+        adc     r11, qword ptr [rsp - 48]
+        add     r13, qword ptr [rsp - 104]
+        adc     r11, qword ptr [rsp - 80]
+        add     r14, qword ptr [rsp - 32]
+        adc     r8, qword ptr [rsp - 24]
+        add     r14, qword ptr [rsp - 88]
+        adc     r8, qword ptr [rsp - 128]
+        add     r12, qword ptr [rsp - 40]
+        adc     r10, qword ptr [rsp - 8]
+        add     r12, qword ptr [rsp - 96]
+        adc     r10, qword ptr [rsp - 112]
+        add     rbx, qword ptr [rsp - 16]
+        adc     rcx, qword ptr [rsp]
+        add     rbx, qword ptr [rsp - 120]
+        adc     rcx, rbp
+        add     rbx, r15
+        adc     rcx, 0
+        shld    rcx, rbx, 13
+        and     rbx, rax
+        add     rcx, r12
+        adc     r10, 0
+        shld    r10, rcx, 13
+        and     rcx, rax
+        add     r10, r14
+        adc     r8, 0
+        shld    r8, r10, 13
+        and     r10, rax
+        add     r8, r13
+        adc     r11, 0
+        shld    r11, r8, 13
+        lea     rdx, [r11 + 8*r11]
+        lea     rdx, [r11 + 2*rdx]
+        add     rdx, r9
+        mov     rsi, rdx
+        shr     rsi, 51
+        add     rsi, rbx
+        mov     r9, rsi
+        shr     r9, 51
+        add     r9, rcx
+        and     r8, rax
+        and     rdx, rax
+        and     rsi, rax
+        mov     qword ptr [rdi], rdx
+        mov     qword ptr [rdi + 8], rsi
+        mov     qword ptr [rdi + 16], r9
+        mov     qword ptr [rdi + 24], r10
+        mov     qword ptr [rdi + 32], r8
+        add     rsp, 8
+        pop     rbx
+        pop     r12
+        pop     r13
+        pop     r14
+        pop     r15
+        pop     rbp
+        ret
+
+_Z29fiat_25519_carry_scmul_121666PmPKm:
+        push    r15
+        push    r14
+        push    r12
+        push    rbx
+        mov     eax, 121666
+        mul     qword ptr [rsi + 32]
+        mov     r8, rdx
+        mov     r10, rax
+        mov     eax, 121666
+        mul     qword ptr [rsi + 24]
+        mov     rcx, rdx
+        mov     r11, rax
+        mov     eax, 121666
+        mul     qword ptr [rsi + 16]
+        mov     r14, rdx
+        mov     rbx, rax
+        mov     eax, 121666
+        mul     qword ptr [rsi + 8]
+        mov     r15, rax
+        mov     r9, rdx
+        mov     eax, 121666
+        mul     qword ptr [rsi]
+        shld    rdx, rax, 13
+        movabs  rsi, 2251799813685247
+        lea     r12, [rsi - 1]
+        and     r12, rax
+        add     rdx, r15
+        adc     r9, 0
+        shld    r9, rdx, 13
+        and     rdx, rsi
+        add     r9, rbx
+        adc     r14, 0
+        shld    r14, r9, 13
+        and     r9, rsi
+        add     r14, r11
+        adc     rcx, 0
+        shld    rcx, r14, 13
+        and     r14, rsi
+        add     rcx, r10
+        adc     r8, 0
+        shld    r8, rcx, 13
+        and     rcx, rsi
+        lea     rax, [r8 + 8*r8]
+        lea     rax, [r8 + 2*rax]
+        add     rax, r12
+        mov     r8, rax
+        shr     r8, 51
+        and     rax, rsi
+        movzx   r8d, r8b
+        add     r8, rdx
+        mov     rdx, r8
+        shr     rdx, 51
+        add     rdx, r9
+        and     r8, rsi
+        mov     qword ptr [rdi], rax
+        mov     qword ptr [rdi + 8], r8
+        mov     qword ptr [rdi + 16], rdx
+        mov     qword ptr [rdi + 24], r14
+        mov     qword ptr [rdi + 32], rcx
+        pop     rbx
+        pop     r12
+        pop     r14
+        pop     r15
+        ret
+
+_Z16fiat_25519_carryPmPKm:
+        mov     r9, qword ptr [rsi]
+        mov     rcx, r9
+        shr     rcx, 51
+        add     rcx, qword ptr [rsi + 8]
+        mov     rax, rcx
+        shr     rax, 51
+        add     rax, qword ptr [rsi + 16]
+        mov     rdx, rax
+        shr     rdx, 51
+        add     rdx, qword ptr [rsi + 24]
+        mov     r8, rdx
+        shr     r8, 51
+        add     r8, qword ptr [rsi + 32]
+        movabs  rsi, 2251799813685247
+        and     r9, rsi
+        mov     r10, r8
+        shr     r10, 51
+        lea     r11, [r10 + 8*r10]
+        lea     r10, [r10 + 2*r11]
+        add     r10, r9
+        mov     r9, r10
+        shr     r9, 51
+        and     rcx, rsi
+        add     rcx, r9
+        and     r10, rsi
+        mov     r9, rcx
+        and     r9, rsi
+        shr     rcx, 51
+        and     rax, rsi
+        add     rax, rcx
+        and     rdx, rsi
+        and     r8, rsi
+        mov     qword ptr [rdi], r10
+        mov     qword ptr [rdi + 8], r9
+        mov     qword ptr [rdi + 16], rax
+        mov     qword ptr [rdi + 24], rdx
+        mov     qword ptr [rdi + 32], r8
+        ret
+
+_Z14fiat_25519_addPmPKmS1_:
+        mov     rax, qword ptr [rdx]
+        mov     rcx, qword ptr [rdx + 8]
+        add     rax, qword ptr [rsi]
+        add     rcx, qword ptr [rsi + 8]
+        mov     r8, qword ptr [rdx + 16]
+        add     r8, qword ptr [rsi + 16]
+        mov     r9, qword ptr [rdx + 24]
+        add     r9, qword ptr [rsi + 24]
+        mov     rdx, qword ptr [rdx + 32]
+        add     rdx, qword ptr [rsi + 32]
+        mov     qword ptr [rdi], rax
+        mov     qword ptr [rdi + 8], rcx
+        mov     qword ptr [rdi + 16], r8
+        mov     qword ptr [rdi + 24], r9
+        mov     qword ptr [rdi + 32], rdx
+        ret
+
+_Z14fiat_25519_subPmPKmS1_:
+        movabs  rax, 4503599627370494
+        mov     rcx, qword ptr [rsi]
+        add     rcx, rax
+        sub     rcx, qword ptr [rdx]
+        mov     r8, qword ptr [rsi + 8]
+        add     r8, rax
+        sub     r8, qword ptr [rdx + 8]
+        mov     r9, qword ptr [rsi + 16]
+        add     r9, rax
+        sub     r9, qword ptr [rdx + 16]
+        mov     r10, qword ptr [rsi + 24]
+        add     r10, rax
+        sub     r10, qword ptr [rdx + 24]
+        add     rax, qword ptr [rsi + 32]
+        add     rcx, -36
+        sub     rax, qword ptr [rdx + 32]
+        mov     qword ptr [rdi], rcx
+        mov     qword ptr [rdi + 8], r8
+        mov     qword ptr [rdi + 16], r9
+        mov     qword ptr [rdi + 24], r10
+        mov     qword ptr [rdi + 32], rax
+        ret
+
+_Z14fiat_25519_oppPmPKm:
+        movabs  rax, 4503599627370494
+        mov     rcx, rax
+        sub     rcx, qword ptr [rsi]
+        mov     rdx, rax
+        sub     rdx, qword ptr [rsi + 8]
+        mov     r8, rax
+        sub     r8, qword ptr [rsi + 16]
+        mov     r9, rax
+        sub     r9, qword ptr [rsi + 24]
+        add     rcx, -36
+        sub     rax, qword ptr [rsi + 32]
+        mov     qword ptr [rdi], rcx
+        mov     qword ptr [rdi + 8], rdx
+        mov     qword ptr [rdi + 16], r8
+        mov     qword ptr [rdi + 24], r9
+        mov     qword ptr [rdi + 32], rax
+        ret
+
+_Z20fiat_25519_selectznzPmhPKmS1_:
+        push    r15
+        push    r14
+        push    rbx
+        lea     rax, [rdx + 8]
+        lea     r8, [rcx + 8]
+        lea     r9, [rdx + 16]
+        lea     r10, [rcx + 16]
+        lea     r11, [rdx + 24]
+        lea     rbx, [rcx + 24]
+        lea     r14, [rdx + 32]
+        lea     r15, [rcx + 32]
+        test    esi, esi
+        cmove   rcx, rdx
+        cmove   r8, rax
+        mov     rax, qword ptr [rcx]
+        mov     rcx, qword ptr [r8]
+        cmove   r10, r9
+        mov     rdx, qword ptr [r10]
+        cmove   rbx, r11
+        mov     rsi, qword ptr [rbx]
+        cmove   r15, r14
+        mov     r8, qword ptr [r15]
+        mov     qword ptr [rdi], rax
+        mov     qword ptr [rdi + 8], rcx
+        mov     qword ptr [rdi + 16], rdx
+        mov     qword ptr [rdi + 24], rsi
+        mov     qword ptr [rdi + 32], r8
+        pop     rbx
+        pop     r14
+        pop     r15
+        ret
+
+_Z19fiat_25519_to_bytesPhPKm:
+        push    rbp
+        push    r15
+        push    r14
+        push    r13
+        push    r12
+        push    rbx
+        mov     rax, qword ptr [rsi]
+        movabs  r9, -2251799813685247
+        add     rax, r9
+        add     rax, 18
+        movabs  r11, 2251799813685247
+        mov     r10, rax
+        and     r10, r11
+        shr     rax, 51
+        neg     eax
+        movzx   eax, al
+        mov     rcx, qword ptr [rsi + 8]
+        add     rcx, r9
+        sub     rcx, rax
+        mov     rax, rcx
+        and     rax, r11
+        shr     rcx, 51
+        neg     ecx
+        movzx   ecx, cl
+        mov     rdx, qword ptr [rsi + 16]
+        add     rdx, r9
+        sub     rdx, rcx
+        mov     r8, rdx
+        and     r8, r11
+        shr     rdx, 51
+        neg     edx
+        movzx   ecx, dl
+        mov     rbx, qword ptr [rsi + 24]
+        add     rbx, r9
+        sub     rbx, rcx
+        mov     rdx, rbx
+        and     rdx, r11
+        shr     rbx, 51
+        neg     ebx
+        add     r9, qword ptr [rsi + 32]
+        movzx   ecx, bl
+        sub     r9, rcx
+        movabs  rcx, 574208952489738240
+        and     rcx, r9
+        lea     rbx, [r11 - 18]
+        test    rcx, rcx
+        cmove   rbx, rcx
+        cmovne  rcx, r11
+        add     rbx, r10
+        mov     r10, rbx
+        mov     rsi, rbx
+        shr     rsi, 51
+        add     rax, rcx
+        add     rax, rsi
+        mov     rsi, rax
+        shr     rsi, 51
+        add     r8, rcx
+        add     r8, rsi
+        mov     rsi, r8
+        shr     rsi, 51
+        add     rdx, rcx
+        add     rdx, rsi
+        mov     rsi, rdx
+        shr     rsi, 51
+        add     rcx, r9
+        add     rcx, rsi
+        mov     ebp, ecx
+        shl     ebp, 4
+        mov     esi, r8d
+        shl     esi, 6
+        shr     r10, 48
+        and     r10d, 7
+        lea     r9d, [r10 + 8*rax]
+        mov     dword ptr [rsp - 20], r9d
+        mov     dword ptr [rsp - 24], eax
+        mov     dword ptr [rsp - 28], eax
+        mov     dword ptr [rsp - 32], eax
+        mov     qword ptr [rsp - 8], rax
+        mov     qword ptr [rsp - 16], rax
+        shr     rax, 45
+        and     eax, 63
+        or      eax, esi
+        mov     dword ptr [rsp - 36], r8d
+        mov     dword ptr [rsp - 40], r8d
+        mov     r13d, r8d
+        mov     r12, r8
+        mov     r15, r8
+        mov     r14, r8
+        shr     r8, 50
+        and     r8d, 1
+        lea     esi, [r8 + 2*rdx]
+        mov     dword ptr [rsp - 44], esi
+        mov     r11d, edx
+        mov     r10d, edx
+        mov     r9d, edx
+        mov     r8, rdx
+        mov     rsi, rdx
+        shr     rdx, 47
+        and     edx, 15
+        or      edx, ebp
+        mov     byte ptr [rdi], bl
+        mov     byte ptr [rdi + 1], bh
+        mov     ebp, ebx
+        shr     ebp, 16
+        mov     byte ptr [rdi + 2], bpl
+        mov     ebp, ebx
+        shr     ebp, 24
+        mov     byte ptr [rdi + 3], bpl
+        mov     rbp, rbx
+        shr     rbp, 32
+        mov     byte ptr [rdi + 4], bpl
+        shr     rbx, 40
+        mov     byte ptr [rdi + 5], bl
+        mov     ebx, dword ptr [rsp - 20]
+        mov     byte ptr [rdi + 6], bl
+        mov     ebx, dword ptr [rsp - 24]
+        shr     ebx, 5
+        mov     byte ptr [rdi + 7], bl
+        mov     ebx, dword ptr [rsp - 28]
+        shr     ebx, 13
+        mov     byte ptr [rdi + 8], bl
+        mov     ebx, dword ptr [rsp - 32]
+        shr     ebx, 21
+        mov     byte ptr [rdi + 9], bl
+        mov     rbx, qword ptr [rsp - 8]
+        shr     rbx, 29
+        mov     byte ptr [rdi + 10], bl
+        mov     rbx, qword ptr [rsp - 16]
+        shr     rbx, 37
+        mov     byte ptr [rdi + 11], bl
+        mov     byte ptr [rdi + 12], al
+        mov     eax, dword ptr [rsp - 36]
+        shr     eax, 2
+        mov     byte ptr [rdi + 13], al
+        mov     eax, dword ptr [rsp - 40]
+        shr     eax, 10
+        mov     byte ptr [rdi + 14], al
+        shr     r13d, 18
+        mov     byte ptr [rdi + 15], r13b
+        shr     r12, 26
+        mov     byte ptr [rdi + 16], r12b
+        shr     r15, 34
+        mov     byte ptr [rdi + 17], r15b
+        shr     r14, 42
+        mov     byte ptr [rdi + 18], r14b
+        mov     eax, dword ptr [rsp - 44]
+        mov     byte ptr [rdi + 19], al
+        shr     r11d, 7
+        mov     byte ptr [rdi + 20], r11b
+        shr     r10d, 15
+        mov     byte ptr [rdi + 21], r10b
+        shr     r9d, 23
+        mov     byte ptr [rdi + 22], r9b
+        shr     r8, 31
+        mov     byte ptr [rdi + 23], r8b
+        shr     rsi, 39
+        mov     byte ptr [rdi + 24], sil
+        mov     byte ptr [rdi + 25], dl
+        mov     eax, ecx
+        shr     eax, 4
+        mov     byte ptr [rdi + 26], al
+        mov     eax, ecx
+        shr     eax, 12
+        mov     byte ptr [rdi + 27], al
+        mov     eax, ecx
+        shr     eax, 20
+        mov     byte ptr [rdi + 28], al
+        mov     rax, rcx
+        shr     rax, 28
+        mov     byte ptr [rdi + 29], al
+        mov     rax, rcx
+        shr     rax, 36
+        mov     byte ptr [rdi + 30], al
+        shr     rcx, 44
+        and     cl, 127
+        mov     byte ptr [rdi + 31], cl
+        pop     rbx
+        pop     r12
+        pop     r13
+        pop     r14
+        pop     r15
+        pop     rbp
+        ret
+
+_Z21fiat_25519_from_bytesPmPKh:
+        push    r14
+        push    rbx
+        movzx   eax, byte ptr [rsi + 31]
+        shl     rax, 44
+        movzx   ecx, byte ptr [rsi + 30]
+        shl     rcx, 36
+        or      rcx, rax
+        movzx   eax, byte ptr [rsi + 29]
+        shl     rax, 28
+        or      rax, rcx
+        movzx   ecx, byte ptr [rsi + 28]
+        shl     ecx, 20
+        or      rcx, rax
+        movzx   edx, byte ptr [rsi + 27]
+        shl     edx, 12
+        or      rdx, rcx
+        movzx   eax, byte ptr [rsi + 26]
+        shl     eax, 4
+        or      rax, rdx
+        movzx   ecx, byte ptr [rsi + 25]
+        shl     rcx, 47
+        movzx   edx, byte ptr [rsi + 24]
+        shl     rdx, 39
+        or      rdx, rcx
+        movzx   ecx, byte ptr [rsi + 23]
+        shl     rcx, 31
+        or      rcx, rdx
+        movzx   edx, byte ptr [rsi + 22]
+        shl     edx, 23
+        or      rdx, rcx
+        movzx   r8d, byte ptr [rsi + 21]
+        shl     r8d, 15
+        or      r8, rdx
+        movzx   ecx, byte ptr [rsi + 20]
+        shl     ecx, 7
+        or      rcx, r8
+        movzx   edx, byte ptr [rsi + 19]
+        shl     rdx, 50
+        movzx   r8d, byte ptr [rsi + 18]
+        shl     r8, 42
+        or      r8, rdx
+        movzx   edx, byte ptr [rsi + 17]
+        shl     rdx, 34
+        or      rdx, r8
+        movzx   r8d, byte ptr [rsi + 16]
+        shl     r8, 26
+        or      r8, rdx
+        movzx   r9d, byte ptr [rsi + 15]
+        shl     r9d, 18
+        or      r9, r8
+        movzx   edx, byte ptr [rsi + 14]
+        shl     edx, 10
+        or      rdx, r9
+        movzx   r8d, byte ptr [rsi + 13]
+        movzx   r9d, byte ptr [rsi + 12]
+        shl     r9, 45
+        movzx   r10d, byte ptr [rsi + 11]
+        shl     r10, 37
+        or      r10, r9
+        movzx   r9d, byte ptr [rsi + 10]
+        shl     r9, 29
+        or      r9, r10
+        movzx   r10d, byte ptr [rsi + 9]
+        shl     r10d, 21
+        or      r10, r9
+        movzx   r11d, byte ptr [rsi + 8]
+        shl     r11d, 13
+        or      r11, r10
+        movzx   r9d, byte ptr [rsi + 7]
+        shl     r9d, 5
+        or      r9, r11
+        movzx   r10d, byte ptr [rsi + 6]
+        shl     r10, 48
+        movzx   r11d, byte ptr [rsi + 5]
+        shl     r11, 40
+        movzx   ebx, byte ptr [rsi + 4]
+        shl     rbx, 32
+        or      rbx, r11
+        movzx   r11d, byte ptr [rsi + 3]
+        shl     r11d, 24
+        or      r11, rbx
+        movzx   ebx, byte ptr [rsi + 2]
+        shl     ebx, 16
+        or      rbx, r11
+        movzx   r11d, byte ptr [rsi + 1]
+        shl     r11d, 8
+        movzx   r14d, byte ptr [rsi]
+        or      r14, rbx
+        or      r14, r11
+        add     r14, r10
+        movabs  rsi, 2251799813685247
+        mov     r10, r14
+        and     r10, rsi
+        shr     r14, 51
+        movzx   r11d, r14b
+        add     r11, r9
+        mov     r9, r11
+        and     r9, rsi
+        shr     r11, 51
+        movzx   r11d, r11b
+        lea     rdx, [rdx + 4*r8]
+        add     rdx, r11
+        mov     r8, rdx
+        and     r8, rsi
+        shr     rdx, 51
+        movzx   edx, dl
+        add     rdx, rcx
+        and     rsi, rdx
+        shr     rdx, 51
+        movzx   ecx, dl
+        add     rcx, rax
+        mov     qword ptr [rdi], r10
+        mov     qword ptr [rdi + 8], r9
+        mov     qword ptr [rdi + 16], r8
+        mov     qword ptr [rdi + 24], rsi
+        mov     qword ptr [rdi + 32], rcx
+        pop     rbx
+        pop     r14
+        ret
