src/Assembly/Parse/Examples/make-example.sh
@@ -1,0 +1,15 @@
+#!/bin/sh
+
+cat << EOF
+From Coq Require Import String List.
+Import ListNotations.
+Local Open Scope string_scope.
+Local Open Scope list_scope.
+Example example : list string := [
+EOF
+
+while read -r line; do
+  echo "\"$line\";"
+done
+
+echo '""].'
